theories/FOL/Arithmetics/DeductionFacts.v
@@ -30,7 +30,7 @@ Section FA_prv.
     apply (Weak FAeq).
 
     pose (sigma := [t] ∗ var ).
-    change (FAeq ⊢ _) with (FAeq ⊢ ($0 == $0)[sigma]).
+    change (FAeq ⊢ _) with (FAeq ⊢ ($0 == $0).[sigma]).
     
     eapply subst_forall_prv with 1.
     apply Ctx. all : firstorder.
@@ -43,7 +43,7 @@ Section FA_prv.
     apply IE. apply (Weak FAeq).
 
     pose (sigma := [x ; y] ∗ var ).
-    change (FAeq ⊢ _) with (FAeq ⊢ ($1 == $0 → $0 == $1)[sigma]).
+    change (FAeq ⊢ _) with (FAeq ⊢ ($1 == $0 → $0 == $1).[sigma]).
     
     eapply subst_forall_prv with 2.
     apply Ctx. all : firstorder.
@@ -58,7 +58,7 @@ Section FA_prv.
     apply Weak with FAeq.
 
     pose (sigma := [x ; y ; z] ∗ var).
-    change (FAeq ⊢ _) with (FAeq ⊢ ($2 == $1 → $1 == $0 → $2 == $0)[sigma]).
+    change (FAeq ⊢ _) with (FAeq ⊢ ($2 == $1 → $1 == $0 → $2 == $0).[sigma]).
     
     eapply subst_forall_prv with 3.
     apply Ctx. all : try firstorder.
@@ -71,7 +71,7 @@ Section FA_prv.
     apply IE. apply Weak with FAeq.
 
     pose (sigma := [y ; x] ∗ var ).
-    change (FAeq ⊢ _) with (FAeq ⊢ ($0 == $1 → σ $0 == σ $1)[sigma]).
+    change (FAeq ⊢ _) with (FAeq ⊢ ($0 == $1 → σ $0 == σ $1).[sigma]).
 
     eapply subst_forall_prv with 2.
     apply Ctx. all : firstorder.
@@ -86,7 +86,7 @@ Section FA_prv.
     apply Weak with FAeq.
 
     pose (sigma := [y2 ; y1 ; x2 ; x1] ∗ var).
-    change (FAeq ⊢ _) with (FAeq ⊢ ($0 == $1 → $2 == $3 → $0 ⊕ $2 == $1 ⊕ $3)[sigma]).
+    change (FAeq ⊢ _) with (FAeq ⊢ ($0 == $1 → $2 == $3 → $0 ⊕ $2 == $1 ⊕ $3).[sigma]).
 
     eapply subst_forall_prv with 4.
     apply Ctx. all: firstorder.
@@ -101,7 +101,7 @@ Section FA_prv.
     apply Weak with FAeq.
     
     pose (sigma := [y2 ; y1 ; x2 ; x1] ∗ var).
-    change (FAeq ⊢ _) with (FAeq ⊢ ($0 == $1 → $2 == $3 → $0 ⊗ $2 == $1 ⊗ $3)[sigma]).
+    change (FAeq ⊢ _) with (FAeq ⊢ ($0 == $1 → $2 == $3 → $0 ⊗ $2 == $1 ⊗ $3).[sigma]).
     
     eapply subst_forall_prv with 4.
     apply Ctx. all: firstorder.
@@ -114,7 +114,7 @@ Section FA_prv.
     apply Weak with FAeq.
 
     pose (sigma := [y ; x] ∗ var).
-    change (FAeq ⊢ _) with (FAeq ⊢ (σ $0 ⊕ $1 == σ ($0 ⊕ $1))[sigma]).
+    change (FAeq ⊢ _) with (FAeq ⊢ (σ $0 ⊕ $1 == σ ($0 ⊕ $1)).[sigma]).
 
     eapply subst_forall_prv with 2.
     apply Ctx. all : firstorder.
@@ -140,7 +140,7 @@ Section FA_prv.
     apply Weak with FAeq.
 
     pose (sigma := [x ; y] ∗ var).
-    change (FAeq ⊢ _) with (FAeq ⊢ ((σ $1) ⊗ $0 == $0 ⊕ ($1 ⊗ $0))[sigma]).
+    change (FAeq ⊢ _) with (FAeq ⊢ ((σ $1) ⊗ $0 == $0 ⊕ ($1 ⊗ $0)).[sigma]).
 
     eapply subst_forall_prv with 2.
     apply Ctx. all : firstorder.
