theories/FOL/Deduction/FullNDFacts.v
@@ -31,7 +31,7 @@ Section ND_def.
   Hint Constructors prv : core.
 
   Theorem subst_Weak A phi xi :
-    A ⊢ phi -> [phi[xi] | phi ∈ A] ⊢ phi[xi].
+    A ⊢ phi -> [phi.[xi] | phi ∈ A] ⊢ phi.[xi].
   Proof.
     induction 1 in xi |-*; comp.
     1-2,7-15: eauto using in_map.
@@ -52,20 +52,20 @@ Section ND_def.
     if Dec (n = x) then $0 else $(S x).
 
   Lemma cycle_shift_shift n phi :
-    bounded n phi -> phi[cycle_shift n] = phi[↑].
+    bounded n phi -> phi.[cycle_shift n] = phi.[↑].
   Proof.
     intros H. apply (bounded_subst H). intros k. unfold cycle_shift. decide _; trivial; lia.
   Qed.
 
   Lemma cycle_shift_subject n phi :
-    bounded (S n) phi -> phi[$n..][cycle_shift n] = phi.
+    bounded (S n) phi -> phi.[$n..].[cycle_shift n] = phi.
   Proof.
     intros H. erewrite subst_comp, (bounded_subst H), subst_id; trivial.
     intros []; cbn; unfold cycle_shift; decide _; trivial; lia.
   Qed.
 
   Lemma nameless_equiv_all' A phi n :
-    bounded_L n A -> bounded (S n) phi -> [p[↑] | p ∈ A] ⊢ phi <-> A ⊢ phi[$n..].
+    bounded_L n A -> bounded (S n) phi -> [p.[↑] | p ∈ A] ⊢ phi <-> A ⊢ phi.[$n..].
   Proof.
     intros H1 H2. split; intros H.
     - apply (subst_Weak ($n..)) in H. rewrite map_map in *.
@@ -76,7 +76,7 @@ Section ND_def.
   Qed.
 
   Lemma nameless_equiv_ex' A phi psi n :
-    bounded_L n A -> bounded n phi -> bounded (S n) psi -> (psi::[p0[↑] | p0 ∈ A]) ⊢ phi[↑] <-> (psi[$n..]::A) ⊢ phi.
+    bounded_L n A -> bounded n phi -> bounded (S n) psi -> (psi::[p0.[↑] | p0 ∈ A]) ⊢ phi.[↑] <-> (psi.[$n..]::A) ⊢ phi.
   Proof.
     intros HL Hphi Hpsi. split.
     - intros H % (subst_Weak ($n..)). cbn in *.
@@ -90,7 +90,7 @@ Section ND_def.
   Qed.
 
   Lemma nameless_equiv_all A phi :
-    { t : term | map (subst_form ↑) A ⊢ phi <-> A ⊢ phi[t..] }.
+    { t : term | map (subst_form ↑) A ⊢ phi <-> A ⊢ phi.[t..] }.
   Proof.
     destruct (find_bounded_L (phi::A)) as [n H].
     exists $n. apply nameless_equiv_all'.
@@ -99,7 +99,7 @@ Section ND_def.
   Qed.
 
   Lemma nameless_equiv_ex A phi psi :
-    { t : term | (phi :: map (subst_form ↑) A) ⊢ psi[↑] <-> (phi[t..]::A) ⊢ psi }.
+    { t : term | (phi :: map (subst_form ↑) A) ⊢ psi.[↑] <-> (phi.[t..]::A) ⊢ psi }.
   Proof.
     destruct (find_bounded_L (phi::psi::A)) as [n H].
     exists $n. apply nameless_equiv_ex'.
@@ -109,7 +109,7 @@ Section ND_def.
   Qed.
 
   Lemma AllI_named (A : list form) (phi : form) :
-    (forall t, A ⊢ phi[t..]) -> A ⊢ ∀phi.
+    (forall t, A ⊢ phi.[t..]) -> A ⊢ ∀phi.
   Proof.
     intros H. apply AllI. 
     destruct (nameless_equiv_all A phi) as [t Ht].
@@ -117,7 +117,7 @@ Section ND_def.
   Qed.
 
   Lemma ExE_named A χ ψ :
-    A ⊢ ∃ χ -> (forall t, (χ[t..]::A) ⊢ ψ) -> A ⊢ ψ.
+    A ⊢ ∃ χ -> (forall t, (χ.[t..]::A) ⊢ ψ) -> A ⊢ ψ.
   Proof.
     intros H1 H2. destruct (nameless_equiv_ex A χ ψ) as [t Ht].
     eapply ExE.
@@ -171,7 +171,7 @@ Section ND_def.
   Qed.
 
   Lemma subst_exist_prv {sigma N Gamma} phi :
-    Gamma ⊢ phi[sigma] -> bounded N phi -> Gamma ⊢ exist_times N phi. 
+    Gamma ⊢ phi.[sigma] -> bounded N phi -> Gamma ⊢ exist_times N phi. 
   Proof.
     induction N in phi, sigma |-*; intros; cbn.
     - erewrite <- (subst_bounded 0); eassumption.
@@ -182,7 +182,7 @@ Section ND_def.
   Qed.
   
   Lemma subst_forall_prv phi {N Gamma} :
-    Gamma ⊢ (forall_times N phi) -> bounded N phi -> forall sigma, Gamma ⊢ phi[sigma].
+    Gamma ⊢ (forall_times N phi) -> bounded N phi -> forall sigma, Gamma ⊢ phi.[sigma].
   Proof.
     induction N in phi |-*; intros ?? sigma; cbn in *.
     - change sigma with (iter up 0 sigma).
@@ -225,13 +225,13 @@ Lemma prv_ind_full {Σ_funcs : funcs_signature} {Σ_preds : preds_signature} :
     (forall (p : peirce) (A : list form) (phi : form),
         (map (subst_form ↑) A) ⊢ phi -> P p (map (subst_form ↑) A) phi -> P p A (∀ phi)) ->
     (forall (p : peirce) (A : list form) (t : term) (phi : form),
-        A ⊢ ∀ phi -> P p A (∀ phi) -> P p A phi[t..]) ->
+        A ⊢ ∀ phi -> P p A (∀ phi) -> P p A phi.[t..]) ->
     (forall (p : peirce) (A : list form) (t : term) (phi : form),
-        A ⊢ phi[t..] -> P p A phi[t..] -> P p A (∃ phi)) ->
+        A ⊢ phi.[t..] -> P p A phi.[t..] -> P p A (∃ phi)) ->
     (forall (p : peirce) (A : list form) (phi psi : form),
         A ⊢ ∃ phi ->
               P p A (∃ phi) ->
-              (phi :: [p[↑] | p ∈ A]) ⊢ psi[↑] -> P p (phi :: [p[↑] | p ∈ A]) psi[↑] -> P p A psi) ->
+              (phi :: [p.[↑] | p ∈ A]) ⊢ psi.[↑] -> P p (phi :: [p.[↑] | p ∈ A]) psi.[↑] -> P p A psi) ->
     (forall (p : peirce) (A : list form) (phi : form), A ⊢ ⊥ -> P p A ⊥ -> P p A phi) ->
     (forall (p : peirce) (A : list form) (phi : form), phi el A -> P p A phi) ->
     (forall (p : peirce) (A : list form) (phi psi : form),
@@ -355,10 +355,10 @@ Section Enumerability.
     (* II *)   concat ([ [ phi → psi | psi ∈ L_ded (phi :: A) n ] | phi ∈ L_T form n ]) ++
     (* IE *)   [ psi | (phi, psi) ∈ (L_ded A n × L_T form n) , (phi → psi el L_ded A n) ] ++
     (* AllI *) [ ∀ phi | phi ∈ L_ded (map (subst_form ↑) A) n ] ++
-    (* AllE *) [ phi[t..] | (phi, t) ∈ (L_T form n × L_T term n), (∀ phi) el L_ded A n ] ++
-    (* ExI *)  [ ∃ phi | (phi, t) ∈ (L_T form n × L_T term n), (phi[t..]) el L_ded A n ] ++
+    (* AllE *) [ phi.[t..] | (phi, t) ∈ (L_T form n × L_T term n), (∀ phi) el L_ded A n ] ++
+    (* ExI *)  [ ∃ phi | (phi, t) ∈ (L_T form n × L_T term n), (phi.[t..]) el L_ded A n ] ++
     (* ExE *)  [ psi | (phi, psi) ∈ (L_T form n × L_T form n),
-                     (∃ phi) el L_ded A n /\ psi[↑] el L_ded (phi::(map (subst_form ↑) A)) n ] ++
+                     (∃ phi) el L_ded A n /\ psi.[↑] el L_ded (phi::(map (subst_form ↑) A)) n ] ++
     (* Exp *)  (match b with falsity_on => fun A =>
                 [ phi | phi ∈ L_T form n, ⊥ el @L_ded _ falsity_on A n ]
                 | _ => fun _ => nil end A) ++
